Up-to bind for CTrees (WIP)

CTree.v
@@ -1,4 +1,14 @@
-From CTree Require Import CTree Eq.
+From RelationAlgebra Require Import
+     kat
+     kat_tac
+     prop
+     rel
+     srel
+     comparisons
+     rewriting
+     normalisation
+     monoid.
+From CTree Require Import CTree Eq Eq.Epsilon.
 From OptSim Require Import Utils LTS OptSim.
 
 Import CoindNotations.
@@ -20,8 +30,8 @@ Program Definition lts {E B X} : LTS :=
   Observable := @olabel E;
   St := @SS E B X;
   LTS.trans := fun l => {| hrel_of := Trans.trans (clabel l) |};
-  epsilon := {| hrel_of := fun _ _ => False |};
-  Robs := eq;
+  (*epsilon := {| hrel_of := fun _ _ => False |};*)
+  Robs := eq; (* FIXME heterogeneous relations *)
   ub_state := fun _ => False
 |}.
 
@@ -31,3 +41,100 @@ Proof.
   intros. cbn. intros.
   eapply (Chain_simF_eq'' (lts := lts)); eauto.
 Qed.
+
+Lemma ObsAnswer_bind_r : forall E B X Y delay R (s' : St (@lts E B Y)) (t : St (@lts E B X)) (k : X -> ctree E B Y) x o,
+  ObsAnswer (lts := lts) delay (fun _ _ => True) Stuck t (oval x) ->
+  ObsAnswer delay R s' (k x) o ->
+  ObsAnswer delay R s' (CTree.bind t k) o.
+Proof.
+  intros. destruct H.
+  - cbn in OBS. subst.
+    destruct H0.
+    + eapply ans_obs; try eassumption. eapply trans_bind_r.
+      apply trans_val_inv in TR as ?. rewrite H in TR. apply TR.
+      apply TR0.
+Admitted.
+
+Lemma epsilon_correct : forall E B X (t u : ctree E B X),
+  Epsilon.epsilon t u ->
+  OptSim.epsilon (lts := lts) t u.
+Proof.
+  red. intros.
+  eapply epsilon_trans; eauto.
+Qed.
+
+Lemma TauAnswer_bind_r : forall E B X Y freeze lock delay (R : Chain (simF freeze lock delay))
+  (s' : St (@lts E B Y)) (t : St (@lts E B X)) (k : X -> ctree E B Y) x,
+  ObsAnswer (lts := lts) delay (fun _ _ => True) Stuck t (oval x) ->
+  TauAnswer freeze delay (`R true) (`R false) s' (k x) ->
+  TauAnswer freeze delay (`R true) (`R false) s' (CTree.bind t k).
+Proof.
+  intros. destruct H.
+  - cbn in OBS. subst.
+    destruct H0.
+    + eapply tau_exact; try eassumption. eapply trans_bind_r.
+      apply trans_val_inv in TR as ?. rewrite H in TR. apply TR.
+      apply TR0.
+    + apply tau_freeze; auto.
+      eapply upto_epsilon_r. admit. 2: apply SIM0.
+      apply epsilon_correct. eapply epsilon_bind_ret.
+      now apply trans_val_epsilon in TR as [].
+    + apply tau_div'; auto. intro.
+      eapply upto_epsilon_r. admit. 2: destruct b; eauto.
+      apply epsilon_correct. eapply epsilon_bind_ret.
+      now apply trans_val_epsilon in TR as [].
+    + eapply tau_delay; try eassumption. admit.
+  - admit.
+Admitted.
+
+Lemma upto_bind E B X Y freeze lock delay : forall
+  (R : Chain (simF (lts := lts) freeze lock delay))
+  b (t t' : ctree E B X) (k k' : X -> ctree E B Y),
+  sim (lts := lts) freeze lock delay b t t' ->
+  (forall x, `R b (k x) (k' x)) ->
+  `R b (CTree.bind t k) (CTree.bind t' k').
+Proof.
+  intro. apply tower. {
+    intros ???????????. apply H; auto.
+    intros. now apply H1.
+  }
+  clear R. intros R **. destruct b.
+  2: { admit. }
+  apply simF_equiv. repeat split; intros.
+  - (* observable transition *)
+    apply trans_bind_inv in H2 as [(? & ? & ? & ?) | (? & ? & ?)].
+    + (* transition from t *)
+      subs. apply sim_fp in H0. apply H0 in H3 as [].
+      * eapply ans_obs. eapply trans_bind_l in TR. apply TR. admit.
+        apply itr_ext_hrel.
+        apply H; auto. apply itr_sim; auto. typeclasses eauto. intros. step. apply H1. apply OBS.
+      * eapply ans_delay_obs; auto. instantiate (1 := (CTree.bind t'0 k')). admit.
+        apply itr_ext_hrel. apply H; auto. intros. apply itr_sim, SIM. typeclasses eauto.
+        intros. step. apply H1.
+    + (* transition from k *)
+      apply sim_fp in H0.
+      eapply ObsAnswer_bind_r.
+      * lapply (proj1 H0 (oval x) Stuck). 2: { apply H2. }
+        intros. eapply ObsAnswer_mon; eauto. cbn. auto.
+      * specialize (H1 x). apply simF_equiv in H1. apply (proj1 H1 o s'). apply H3.
+  - (* tau transition *)
+    apply trans_bind_inv in H2 as [(? & ? & ? & ?) | (? & ? & ?)].
+    + (* transition from t *)
+      subs. apply sim_fp in H0. apply H0 in H3 as [].
+      * eapply tau_exact. eapply trans_bind_l in TR. apply TR. admit.
+        apply H; auto. intros. step. apply H1.
+      * apply tau_freeze; auto.
+        apply H; auto. intros. step. apply H1.
+      * apply tau_div; auto. (* TODO simF_step_t *)
+        apply H; auto. intros. step. apply H1.
+        apply H; auto. intros. apply simF_f_t. now subst. apply H1.
+      * eapply tau_delay; auto. instantiate (1 := (CTree.bind t'0 k')). admit.
+        apply H; auto. intros. step. apply H1.
+    + (* transition from k *)
+      apply sim_fp in H0.
+      eapply TauAnswer_bind_r.
+      * lapply (proj1 H0 (oval x) Stuck). 2: { apply H2. }
+        intros. eapply ObsAnswer_mon; eauto. cbn. auto.
+      * specialize (H1 x). apply simF_equiv in H1. apply (proj1 (proj2 H1) s'). apply H3.
+  - admit.
+Admitted.
